Playing around

stlc.v
@@ -1,4 +1,11 @@
+(* 
+ * Reenactment of commit e7ef8a4cafcd21bd17cbf5cd8004e991577a5a26#diff-5e2396245414cb01f14b3b3629da114aL345
+ *)
+
 From mm Require Import util abt.
+
+(* Old stlc.v before any changes *)
+Module old.
 
 Module exprop.
   Inductive t' :=
@@ -338,7 +345,7 @@ Module step.
     induction Star; intros e1.
     - constructor.
     - econstructor; [|apply IHStar].
-      eauto.
+      auto. (* we change to auto to be consistent *)
   Qed.
 
   Lemma star_If :
@@ -476,3 +483,1300 @@ Module context_equiv.
       value.t v2 ->
       v1 = v2.
 End context_equiv.
+
+End old.
+
+(* Stlc.v after adding a single valuet to the beta case. *)
+Module add_valuet_beta.
+
+Module exprop.
+  Inductive t' :=
+  | abs
+  | app
+  | tt
+  | ff
+  | If
+  .
+  Definition t := t'.
+
+  Definition arity (op : t) : arity.t :=
+    match op with
+    | abs => [1]
+    | app => [0; 0]
+    | tt => []
+    | ff => []
+    | If => [0; 0; 0]
+    end.
+
+  Definition eq_dec : forall x y : t, {x = y} + {x <> y}.
+    decide equality.
+  Defined.
+End exprop.
+
+Module type.
+  Inductive t :=
+  | bool
+  | arrow : t -> t -> t
+  .
+End type.
+
+Module expr_abt := abt.abt exprop.
+
+Module expr_ast.
+  Inductive t :=
+  | var (x : nat) : t
+  | abs : t -> t
+  | app : t -> t -> t
+  | tt : t
+  | ff : t
+  | If : t -> t -> t -> t
+  .
+End expr_ast.
+
+Module expr_basis.
+  Module A := expr_abt.
+
+  Import expr_ast.
+  Definition t := t.
+
+  Fixpoint to_abt (ty : t) : A.t :=
+    match ty with
+    | var n => A.var n
+    | abs e' => A.op exprop.abs [A.bind 1 (to_abt e')]
+    | app e1 e2 => A.op exprop.app [A.bind 0 (to_abt e1); A.bind 0 (to_abt e2)]
+    | tt => A.op exprop.tt []
+    | ff => A.op exprop.ff []
+    | If e1 e2 e3 => A.op exprop.If [A.bind 0 (to_abt e1);
+                                            A.bind 0 (to_abt e2);
+                                            A.bind 0 (to_abt e3)]
+    end.
+
+  Fixpoint of_abt (a : A.t) : t :=
+    match a with
+    | A.var n => var n
+    | A.op exprop.abs [A.bind 1 a'] => abs (of_abt a')
+    | A.op exprop.app [A.bind 0 a1; A.bind 0 a2] => app (of_abt a1) (of_abt a2)
+    | A.op exprop.tt [] => tt
+    | A.op exprop.ff [] => ff
+    | A.op exprop.If [A.bind 0 a1; A.bind 0 a2; A.bind 0 a3] =>
+      If (of_abt a1) (of_abt a2) (of_abt a3)
+    | _ => var 0 (* bogus *)
+    end.
+
+  Fixpoint shift c d (e : t) : t :=
+    match e with
+    | var x => var (if x <? c then x else x + d)
+    | abs e' => abs (shift (S c) d e')
+    | app e1 e2 => app (shift c d e1) (shift c d e2)
+    | tt => tt
+    | ff => ff
+    | If e1 e2 e3 => If (shift c d e1) (shift c d e2) (shift c d e3)
+    end.
+
+  Fixpoint subst rho e :=
+    match e with
+    | var x => match nth_error rho x with
+                  | Some e' => e'
+                  | None => e
+                  end
+    | abs e' => abs (subst (var 0 :: map (shift 0 1) rho) e')
+    | app e1 e2 => app (subst rho e1) (subst rho e2)
+    | tt => tt
+    | ff => ff
+    | If e1 e2 e3 => If (subst rho e1) (subst rho e2) (subst rho e3)
+    end.
+
+  Fixpoint wf n e :=
+    match e with
+    | var x => x < n
+    | abs e' => wf (S n) e'
+    | app e1 e2 => wf n e1 /\ wf n e2
+    | tt => True
+    | ff => True
+    | If e1 e2 e3 => wf n e1 /\ wf n e2 /\ wf n e3
+    end.
+
+  Fixpoint identity_subst (n : nat) : list t :=
+    match n with
+    | 0 => []
+    | S n => var 0 :: map (shift 0 1) (identity_subst n)
+    end.
+
+  Lemma ws_to_abt : forall e, A.ws (to_abt e).
+  Proof. A.basis_util.prove_ws_to_abt. Qed.
+
+  Lemma of_to_abt : forall e, of_abt (to_abt e) = e.
+  Proof. A.basis_util.prove_of_to_abt. Qed.
+
+  Lemma to_of_abt : forall a, A.ws a -> to_abt (of_abt a) = a.
+  Proof. A.basis_util.prove_to_of_abt to_abt of_abt. Qed.
+
+  Lemma shift_to_abt_comm : forall e c d, to_abt (shift c d e) = A.shift c d (to_abt e).
+  Proof. A.basis_util.prove_shift_to_abt_comm. Qed.
+
+  Lemma map_shift_to_abt_comm :
+    forall c d rho, map to_abt (map (shift c d) rho) = map (A.shift c d) (map to_abt rho).
+  Proof. A.basis_util.prove_map_shift_to_abt_comm shift_to_abt_comm. Qed.
+
+  Lemma subst_to_abt_comm : forall e rho,
+      to_abt (subst rho e) = A.subst (map to_abt rho) (to_abt e).
+  Proof. A.basis_util.prove_subst_to_abt_comm t map_shift_to_abt_comm. Qed.
+
+  Lemma wf_to_abt : forall e n, wf n e <-> A.wf n (to_abt e).
+  Proof. A.basis_util.prove_wf_to_abt. Qed.
+
+  Lemma identity_subst_to_abt_comm :
+    forall n, List.map to_abt (identity_subst n) = A.identity_subst n.
+  Proof. A.basis_util.prove_identity_subst_to_abt_comm map_shift_to_abt_comm. Qed.
+
+  Definition var := var.
+  Arguments var /.
+  Lemma var_to_abt : forall n, to_abt (var n) = A.var n.
+  Proof. reflexivity. Qed.
+End expr_basis.
+
+Module expr.
+  Include abt.abt_util expr_basis.
+  Notation abs := expr_ast.abs.
+  Notation app := expr_ast.app.
+  Notation tt := expr_ast.tt.
+  Notation ff := expr_ast.ff.
+  Notation If := expr_ast.If.
+End expr.
+
+
+Module has_type.
+  Inductive t : list type.t -> expr.t -> type.t -> Prop :=
+  | var : forall G x ty,
+      List.nth_error G x = Some ty ->
+      t G (expr.var x) ty
+  | tt : forall G,
+      t G expr.tt type.bool
+  | ff : forall G,
+      t G expr.ff type.bool
+  | abs : forall G e ty1 ty2,
+      t (ty1 :: G) e ty2 ->
+      t G (expr.abs e) (type.arrow ty1 ty2)
+  | app : forall G e1 e2 ty1 ty2,
+      t G e1 (type.arrow ty1 ty2) ->
+      t G e2 ty1 ->
+      t G (expr.app e1 e2) ty2
+  | If : forall G e1 e2 e3 ty,
+      t G e1 type.bool ->
+      t G e2 ty -> 
+      t G e3 ty ->
+      t G (expr.If e1 e2 e3) ty
+  .
+
+  Lemma wf :
+    forall G e ty,
+      t G e ty ->
+      expr.wf (List.length G) e.
+  Proof.
+    induction 1; simpl in *; intuition.
+    pose proof nth_error_Some G x. intuition congruence.
+  Qed.
+
+  Lemma shift :
+    forall G e ty,
+      t G e ty ->
+      forall G1 G2 G',
+        G1 ++ G2 = G ->
+        t (G1 ++ G' ++ G2) (expr.shift (List.length G1) (List.length G') e) ty.
+  Proof.
+    induction 1; intros G1 G2 G' E; subst G.
+    - constructor.
+      do_ltb.
+      + now rewrite nth_error_app1 in * by assumption.
+      + rewrite !nth_error_app2 in * by omega.
+        now do_app2_minus.
+    - constructor.
+    - constructor.
+    - cbn [expr.shift].
+      constructor.
+      change (ty1 :: G1 ++ G' ++ G2) with ((ty1 :: G1) ++ G' ++ G2).
+      now apply IHt.
+    - simpl. econstructor.
+      + now apply IHt1.
+      + now apply IHt2.
+    - simpl. econstructor.
+      + now apply IHt1.
+      + now apply IHt2.
+      + now apply IHt3.
+  Qed.
+
+  Lemma shift' :
+    forall G e ty G',
+      t G e ty ->
+      t (G' ++ G) (expr.shift 0 (List.length G') e) ty.
+  Proof.
+    intros.
+    now apply shift with (G := G) (G1 := []).
+  Qed.
+
+  Lemma shift_cons :
+    forall G e ty ty0,
+      t G e ty ->
+      t (ty0 :: G) (expr.shift 0 1 e) ty.
+  Proof.
+    intros.
+    now apply shift' with (G' := [ty0]).
+  Qed.
+
+  Lemma subst :
+    forall G e ty,
+      t G e ty ->
+      forall G' rho,
+        List.Forall2 (t G') rho G ->
+        t G' (expr.subst rho e) ty.
+  Proof.
+    induction 1; intros G' rho F; cbn [expr.subst].
+    - destruct (Forall2_nth_error2 F H) as [z [Hz Ht]].
+      unfold expr.t in *.
+      simpl.
+      now rewrite Hz.
+    - constructor.
+    - constructor.
+    - constructor.
+      apply IHt.
+      constructor.
+      + now constructor.
+      + apply Forall2_map_l.
+        apply Forall2_forall_suff_weak.
+        * now erewrite Forall2_length by eauto.
+        * intros.
+          apply shift_cons.
+          eapply (Forall2_nth_error F); eauto.
+    - econstructor.
+      + now apply IHt1.
+      + now apply IHt2.
+    - econstructor.
+      + now apply IHt1.
+      + now apply IHt2.
+      + now apply IHt3.
+  Qed.
+End has_type.
+
+Module ctx.
+  Definition t := list type.t.
+End ctx.
+
+Module value.
+  Inductive t : expr.t -> Prop :=
+  | tt : t expr.tt
+  | ff : t expr.ff
+  | abs : forall e, t (expr.abs e)
+  .
+End value.
+
+Module step.
+  Inductive t : expr.t -> expr.t -> Prop :=
+  | beta : forall e1 e2,
+      value.t e2 ->
+      t (expr.app (expr.abs e1) e2)
+        (expr.subst [e2] e1)
+  | app1  : forall e1 e1' e2,
+      t e1 e1' ->
+      t (expr.app e1 e2) (expr.app e1' e2)
+  | app2  : forall e1 e2 e2',
+      t e2 e2' ->
+      t (expr.app e1 e2) (expr.app e1 e2')
+  | IfT : forall e2 e3,
+      t (expr.If expr.tt e2 e3) e2
+  | IfF : forall e2 e3,
+      t (expr.If expr.ff e2 e3) e3
+  | If : forall e1 e1' e2 e3,
+      t e1 e1' ->
+      t (expr.If e1 e2 e3) (expr.If e1' e2 e3)
+  .
+  Hint Constructors t.
+
+  Definition star : expr.t -> expr.t -> Prop := clos_refl_trans_n1 _ t.
+
+  Lemma step_l :
+    forall e1 e2 e3,
+      step.t e1 e2 ->
+      step.star e2 e3 ->
+      step.star e1 e3.
+  Proof.
+    intros e1 e2 e3 S Star.
+    apply clos_rt_rtn1.
+    apply clos_rtn1_rt in Star.
+    eapply rt_trans; eauto using rt_step.
+  Qed.
+
+  Lemma star_app1 :
+    forall e1 e1' e2,
+      star e1 e1' ->
+      star (expr.app e1 e2) (expr.app e1' e2).
+  Proof.
+    intros e1 e1' e2 Star.
+    revert e2.
+    induction Star; intros e2.
+    - constructor.
+    - econstructor; [|apply IHStar].
+      eauto.
+  Qed.
+
+  Lemma star_app2 :
+    forall e1 e2 e2',
+      star e2 e2' ->
+      star (expr.app e1 e2) (expr.app e1 e2').
+  Proof.
+    intros e1 e2 e2' Star.
+    revert e1.
+    induction Star; intros e1.
+    - constructor.
+    - econstructor; [|apply IHStar].
+      auto. (* we change to auto to be consistent *)
+  Qed.
+
+  Lemma star_If :
+    forall e1 e1' e2 e3,
+      star e1 e1' ->
+      star (expr.If e1 e2 e3) (expr.If e1' e2 e3).
+  Proof.
+    intros e1 e1' e2 e3 Star.
+    revert e2 e3.
+    induction Star; intros e2 e3.
+    - constructor.
+    - econstructor; [|apply IHStar].
+      eauto.
+  Qed.
+
+  Lemma star_trans :
+    forall e1 e2 e3,
+      star e1 e2 ->
+      star e2 e3 ->
+      star e1 e3.
+  Proof.
+    intros e1 e2 e3 S1 S2.
+    apply clos_rtn1_rt in S1.
+    apply clos_rtn1_rt in S2.
+    apply clos_rt_rtn1.
+    eauto using rt_trans.
+  Qed.
+
+  Lemma star_refl :
+    forall e,
+      star e e.
+  Proof.
+    constructor.
+  Qed.
+
+  Hint Resolve star_app2 star_app1 star_refl.
+
+  Lemma value :
+    forall v,
+      value.t v ->
+      forall e',
+        step.t v e' ->
+        False.
+  Proof.
+    induction 1; intros e' Step; inversion Step; subst.
+  Qed.
+
+  Lemma star_value :
+    forall v e',
+      value.t v ->
+      step.star v e' ->
+      e' = v.
+  Proof.
+    intros v e' Val Star.
+    apply clos_rtn1_rt in Star.
+    apply clos_rt_rt1n in Star.
+    inversion Star; subst; auto.
+    exfalso; eauto using value.
+  Qed.
+End step.
+
+Module context.
+  Inductive t :=
+  | hole
+  | abs : t -> t
+  | app1 : t -> expr.t -> t
+  | app2 : expr.t -> t -> t
+  | If1 : t -> expr.t -> expr.t -> t
+  | If2 : expr.t -> t -> expr.t -> t
+  | If3 : expr.t -> expr.t -> t -> t
+  .
+
+  Fixpoint plug (C : t) (e : expr.t) : expr.t :=
+    match C with
+    | hole => e
+    | abs C' => expr.abs (plug C' e)
+    | app1 C1 e2 => expr.app (plug C1 e) e2
+    | app2 e1 C2 => expr.app e1 (plug C2 e)
+    | If1 C1 e2 e3 => expr.If (plug C1 e) e2 e3
+    | If2 e1 C2 e3 => expr.If e1 (plug C2 e) e3
+    | If3 e1 e2 C3 => expr.If e1 e2 (plug C3 e)
+    end.
+End context.
+
+Module context_has_type.
+  Inductive t : list type.t -> context.t -> list type.t -> type.t -> type.t -> Prop :=
+  | hole : forall G ty, t G context.hole G ty ty
+  | abs : forall G' C G ty ty1' ty2',
+      t (ty1' :: G') C (ty1' :: G) ty ty2' ->
+      t G' (context.abs C) (ty1' :: G) ty (type.arrow ty1' ty2')
+  | app1 : forall G' C G ty ty1' ty2' e,
+      t G' C G ty (type.arrow ty1' ty2') ->
+      has_type.t G' e ty1' ->
+      t G' (context.app1 C e) G ty ty2'
+  | app2 : forall G' C G ty ty1' ty2' e,
+      has_type.t G' e (type.arrow ty1' ty2') ->
+      t G' C G ty ty1' ->
+      t G' (context.app2 e C) G ty ty2'
+  | If1 : forall G' C1 G ty ty' e2 e3,
+      t G' C1 G ty type.bool ->
+      has_type.t G' e2 ty' ->
+      has_type.t G' e3 ty' ->
+      t G' (context.If1 C1 e2 e3) G ty ty'
+  | If2 : forall G' C2 G ty ty' e1 e3,
+      has_type.t G' e1 type.bool ->
+      t G' C2 G ty ty' ->
+      has_type.t G' e3 ty' ->
+      t G' (context.If2 e1 C2 e3) G ty ty'
+  | If3 : forall G' C3 G ty ty' e1 e2,
+      has_type.t G' e1 type.bool ->
+      has_type.t G' e2 ty' ->
+      t G' C3 G ty ty' ->
+      t G' (context.If3 e1 e2 C3) G ty ty'
+  .
+
+  Theorem plug :
+    forall G' C G ty ty',
+      t G' C G ty ty' ->
+      forall e,
+        has_type.t G e ty ->
+        has_type.t G' (context.plug C e) ty'.
+  Proof.
+    induction 1; intros e0 HT0; cbn [context.plug]; try assumption;
+      apply IHt in HT0; econstructor; eauto.
+  Qed.
+End context_has_type.
+
+Module context_equiv.
+  Definition t G e1 e2 ty : Prop :=
+    forall C v1 v2,
+      context_has_type.t [] C G ty type.bool ->
+      step.star (context.plug C e1) v1 ->
+      value.t v1 ->
+      step.star (context.plug C e2) v2 ->
+      value.t v2 ->
+      v1 = v2.
+End context_equiv.
+
+End add_valuet_beta.
+
+(* Stlc.v after another single valuet to the app2 case. *)
+Module add_valuet_app2.
+
+Module exprop.
+  Inductive t' :=
+  | abs
+  | app
+  | tt
+  | ff
+  | If
+  .
+  Definition t := t'.
+
+  Definition arity (op : t) : arity.t :=
+    match op with
+    | abs => [1]
+    | app => [0; 0]
+    | tt => []
+    | ff => []
+    | If => [0; 0; 0]
+    end.
+
+  Definition eq_dec : forall x y : t, {x = y} + {x <> y}.
+    decide equality.
+  Defined.
+End exprop.
+
+Module type.
+  Inductive t :=
+  | bool
+  | arrow : t -> t -> t
+  .
+End type.
+
+Module expr_abt := abt.abt exprop.
+
+Module expr_ast.
+  Inductive t :=
+  | var (x : nat) : t
+  | abs : t -> t
+  | app : t -> t -> t
+  | tt : t
+  | ff : t
+  | If : t -> t -> t -> t
+  .
+End expr_ast.
+
+Module expr_basis.
+  Module A := expr_abt.
+
+  Import expr_ast.
+  Definition t := t.
+
+  Fixpoint to_abt (ty : t) : A.t :=
+    match ty with
+    | var n => A.var n
+    | abs e' => A.op exprop.abs [A.bind 1 (to_abt e')]
+    | app e1 e2 => A.op exprop.app [A.bind 0 (to_abt e1); A.bind 0 (to_abt e2)]
+    | tt => A.op exprop.tt []
+    | ff => A.op exprop.ff []
+    | If e1 e2 e3 => A.op exprop.If [A.bind 0 (to_abt e1);
+                                            A.bind 0 (to_abt e2);
+                                            A.bind 0 (to_abt e3)]
+    end.
+
+  Fixpoint of_abt (a : A.t) : t :=
+    match a with
+    | A.var n => var n
+    | A.op exprop.abs [A.bind 1 a'] => abs (of_abt a')
+    | A.op exprop.app [A.bind 0 a1; A.bind 0 a2] => app (of_abt a1) (of_abt a2)
+    | A.op exprop.tt [] => tt
+    | A.op exprop.ff [] => ff
+    | A.op exprop.If [A.bind 0 a1; A.bind 0 a2; A.bind 0 a3] =>
+      If (of_abt a1) (of_abt a2) (of_abt a3)
+    | _ => var 0 (* bogus *)
+    end.
+
+  Fixpoint shift c d (e : t) : t :=
+    match e with
+    | var x => var (if x <? c then x else x + d)
+    | abs e' => abs (shift (S c) d e')
+    | app e1 e2 => app (shift c d e1) (shift c d e2)
+    | tt => tt
+    | ff => ff
+    | If e1 e2 e3 => If (shift c d e1) (shift c d e2) (shift c d e3)
+    end.
+
+  Fixpoint subst rho e :=
+    match e with
+    | var x => match nth_error rho x with
+                  | Some e' => e'
+                  | None => e
+                  end
+    | abs e' => abs (subst (var 0 :: map (shift 0 1) rho) e')
+    | app e1 e2 => app (subst rho e1) (subst rho e2)
+    | tt => tt
+    | ff => ff
+    | If e1 e2 e3 => If (subst rho e1) (subst rho e2) (subst rho e3)
+    end.
+
+  Fixpoint wf n e :=
+    match e with
+    | var x => x < n
+    | abs e' => wf (S n) e'
+    | app e1 e2 => wf n e1 /\ wf n e2
+    | tt => True
+    | ff => True
+    | If e1 e2 e3 => wf n e1 /\ wf n e2 /\ wf n e3
+    end.
+
+  Fixpoint identity_subst (n : nat) : list t :=
+    match n with
+    | 0 => []
+    | S n => var 0 :: map (shift 0 1) (identity_subst n)
+    end.
+
+  Lemma ws_to_abt : forall e, A.ws (to_abt e).
+  Proof. A.basis_util.prove_ws_to_abt. Qed.
+
+  Lemma of_to_abt : forall e, of_abt (to_abt e) = e.
+  Proof. A.basis_util.prove_of_to_abt. Qed.
+
+  Lemma to_of_abt : forall a, A.ws a -> to_abt (of_abt a) = a.
+  Proof. A.basis_util.prove_to_of_abt to_abt of_abt. Qed.
+
+  Lemma shift_to_abt_comm : forall e c d, to_abt (shift c d e) = A.shift c d (to_abt e).
+  Proof. A.basis_util.prove_shift_to_abt_comm. Qed.
+
+  Lemma map_shift_to_abt_comm :
+    forall c d rho, map to_abt (map (shift c d) rho) = map (A.shift c d) (map to_abt rho).
+  Proof. A.basis_util.prove_map_shift_to_abt_comm shift_to_abt_comm. Qed.
+
+  Lemma subst_to_abt_comm : forall e rho,
+      to_abt (subst rho e) = A.subst (map to_abt rho) (to_abt e).
+  Proof. A.basis_util.prove_subst_to_abt_comm t map_shift_to_abt_comm. Qed.
+
+  Lemma wf_to_abt : forall e n, wf n e <-> A.wf n (to_abt e).
+  Proof. A.basis_util.prove_wf_to_abt. Qed.
+
+  Lemma identity_subst_to_abt_comm :
+    forall n, List.map to_abt (identity_subst n) = A.identity_subst n.
+  Proof. A.basis_util.prove_identity_subst_to_abt_comm map_shift_to_abt_comm. Qed.
+
+  Definition var := var.
+  Arguments var /.
+  Lemma var_to_abt : forall n, to_abt (var n) = A.var n.
+  Proof. reflexivity. Qed.
+End expr_basis.
+
+Module expr.
+  Include abt.abt_util expr_basis.
+  Notation abs := expr_ast.abs.
+  Notation app := expr_ast.app.
+  Notation tt := expr_ast.tt.
+  Notation ff := expr_ast.ff.
+  Notation If := expr_ast.If.
+End expr.
+
+
+Module has_type.
+  Inductive t : list type.t -> expr.t -> type.t -> Prop :=
+  | var : forall G x ty,
+      List.nth_error G x = Some ty ->
+      t G (expr.var x) ty
+  | tt : forall G,
+      t G expr.tt type.bool
+  | ff : forall G,
+      t G expr.ff type.bool
+  | abs : forall G e ty1 ty2,
+      t (ty1 :: G) e ty2 ->
+      t G (expr.abs e) (type.arrow ty1 ty2)
+  | app : forall G e1 e2 ty1 ty2,
+      t G e1 (type.arrow ty1 ty2) ->
+      t G e2 ty1 ->
+      t G (expr.app e1 e2) ty2
+  | If : forall G e1 e2 e3 ty,
+      t G e1 type.bool ->
+      t G e2 ty -> 
+      t G e3 ty ->
+      t G (expr.If e1 e2 e3) ty
+  .
+
+  Lemma wf :
+    forall G e ty,
+      t G e ty ->
+      expr.wf (List.length G) e.
+  Proof.
+    induction 1; simpl in *; intuition.
+    pose proof nth_error_Some G x. intuition congruence.
+  Qed.
+
+  Lemma shift :
+    forall G e ty,
+      t G e ty ->
+      forall G1 G2 G',
+        G1 ++ G2 = G ->
+        t (G1 ++ G' ++ G2) (expr.shift (List.length G1) (List.length G') e) ty.
+  Proof.
+    induction 1; intros G1 G2 G' E; subst G.
+    - constructor.
+      do_ltb.
+      + now rewrite nth_error_app1 in * by assumption.
+      + rewrite !nth_error_app2 in * by omega.
+        now do_app2_minus.
+    - constructor.
+    - constructor.
+    - cbn [expr.shift].
+      constructor.
+      change (ty1 :: G1 ++ G' ++ G2) with ((ty1 :: G1) ++ G' ++ G2).
+      now apply IHt.
+    - simpl. econstructor.
+      + now apply IHt1.
+      + now apply IHt2.
+    - simpl. econstructor.
+      + now apply IHt1.
+      + now apply IHt2.
+      + now apply IHt3.
+  Qed.
+
+  Lemma shift' :
+    forall G e ty G',
+      t G e ty ->
+      t (G' ++ G) (expr.shift 0 (List.length G') e) ty.
+  Proof.
+    intros.
+    now apply shift with (G := G) (G1 := []).
+  Qed.
+
+  Lemma shift_cons :
+    forall G e ty ty0,
+      t G e ty ->
+      t (ty0 :: G) (expr.shift 0 1 e) ty.
+  Proof.
+    intros.
+    now apply shift' with (G' := [ty0]).
+  Qed.
+
+  Lemma subst :
+    forall G e ty,
+      t G e ty ->
+      forall G' rho,
+        List.Forall2 (t G') rho G ->
+        t G' (expr.subst rho e) ty.
+  Proof.
+    induction 1; intros G' rho F; cbn [expr.subst].
+    - destruct (Forall2_nth_error2 F H) as [z [Hz Ht]].
+      unfold expr.t in *.
+      simpl.
+      now rewrite Hz.
+    - constructor.
+    - constructor.
+    - constructor.
+      apply IHt.
+      constructor.
+      + now constructor.
+      + apply Forall2_map_l.
+        apply Forall2_forall_suff_weak.
+        * now erewrite Forall2_length by eauto.
+        * intros.
+          apply shift_cons.
+          eapply (Forall2_nth_error F); eauto.
+    - econstructor.
+      + now apply IHt1.
+      + now apply IHt2.
+    - econstructor.
+      + now apply IHt1.
+      + now apply IHt2.
+      + now apply IHt3.
+  Qed.
+End has_type.
+
+Module ctx.
+  Definition t := list type.t.
+End ctx.
+
+Module value.
+  Inductive t : expr.t -> Prop :=
+  | tt : t expr.tt
+  | ff : t expr.ff
+  | abs : forall e, t (expr.abs e)
+  .
+End value.
+
+Module step.
+  Inductive t : expr.t -> expr.t -> Prop :=
+  | beta : forall e1 e2,
+      value.t e2 ->
+      t (expr.app (expr.abs e1) e2)
+        (expr.subst [e2] e1)
+  | app1  : forall e1 e1' e2,
+      t e1 e1' ->
+      t (expr.app e1 e2) (expr.app e1' e2)
+  | app2  : forall e1 e2 e2',
+      value.t e1 ->
+      t e2 e2' ->
+      t (expr.app e1 e2) (expr.app e1 e2')
+  | IfT : forall e2 e3,
+      t (expr.If expr.tt e2 e3) e2
+  | IfF : forall e2 e3,
+      t (expr.If expr.ff e2 e3) e3
+  | If : forall e1 e1' e2 e3,
+      t e1 e1' ->
+      t (expr.If e1 e2 e3) (expr.If e1' e2 e3)
+  .
+  Hint Constructors t.
+
+  Definition star : expr.t -> expr.t -> Prop := clos_refl_trans_n1 _ t.
+
+  Lemma step_l :
+    forall e1 e2 e3,
+      step.t e1 e2 ->
+      step.star e2 e3 ->
+      step.star e1 e3.
+  Proof.
+    intros e1 e2 e3 S Star.
+    apply clos_rt_rtn1.
+    apply clos_rtn1_rt in Star.
+    eapply rt_trans; eauto using rt_step.
+  Qed.
+
+  Lemma star_app1 :
+    forall e1 e1' e2,
+      star e1 e1' ->
+      star (expr.app e1 e2) (expr.app e1' e2).
+  Proof.
+    intros e1 e1' e2 Star.
+    revert e2.
+    induction Star; intros e2.
+    - constructor.
+    - econstructor; [|apply IHStar].
+      eauto.
+  Qed.
+
+  (* 
+   * As expected, star_app2 breaks.
+   * Like James, we add the premise here.
+   *)
+  Lemma star_app2 :
+    forall e1 e2 e2',
+      value.t e1 -> (* new _ : value.t e1 *)
+      star e2 e2' ->
+      star (expr.app e1 e2) (expr.app e1 e2').
+  Proof.
+    intros e1 e2 e2' Val1 Star. (* new Val1 : value.t eq *)
+    revert e1 Val1. (* need to revert this too, now *)
+    induction Star; intros e1 Val1.
+    - constructor.
+    - econstructor; [|apply IHStar];
+      auto. (* two cases now, note the semicolon *)
+  Qed.
+
+  Lemma star_If :
+    forall e1 e1' e2 e3,
+      star e1 e1' ->
+      star (expr.If e1 e2 e3) (expr.If e1' e2 e3).
+  Proof.
+    intros e1 e1' e2 e3 Star.
+    revert e2 e3.
+    induction Star; intros e2 e3.
+    - constructor.
+    - econstructor; [|apply IHStar].
+      eauto.
+  Qed.
+
+  Lemma star_trans :
+    forall e1 e2 e3,
+      star e1 e2 ->
+      star e2 e3 ->
+      star e1 e3.
+  Proof.
+    intros e1 e2 e3 S1 S2.
+    apply clos_rtn1_rt in S1.
+    apply clos_rtn1_rt in S2.
+    apply clos_rt_rtn1.
+    eauto using rt_trans.
+  Qed.
+
+  Lemma star_refl :
+    forall e,
+      star e e.
+  Proof.
+    constructor.
+  Qed.
+
+  Hint Resolve (*star_app2*) star_app1 star_refl.
+
+  Lemma value :
+    forall v,
+      value.t v ->
+      forall e',
+        step.t v e' ->
+        False.
+  Proof.
+    induction 1; intros e' Step; inversion Step; subst.
+  Qed.
+
+  Lemma star_value :
+    forall v e',
+      value.t v ->
+      step.star v e' ->
+      e' = v.
+  Proof.
+    intros v e' Val Star.
+    apply clos_rtn1_rt in Star.
+    apply clos_rt_rt1n in Star.
+    inversion Star; subst; auto.
+    exfalso; eauto using value.
+  Qed.
+End step.
+
+Module context.
+  Inductive t :=
+  | hole
+  | abs : t -> t
+  | app1 : t -> expr.t -> t
+  | app2 : expr.t -> t -> t
+  | If1 : t -> expr.t -> expr.t -> t
+  | If2 : expr.t -> t -> expr.t -> t
+  | If3 : expr.t -> expr.t -> t -> t
+  .
+
+  Fixpoint plug (C : t) (e : expr.t) : expr.t :=
+    match C with
+    | hole => e
+    | abs C' => expr.abs (plug C' e)
+    | app1 C1 e2 => expr.app (plug C1 e) e2
+    | app2 e1 C2 => expr.app e1 (plug C2 e)
+    | If1 C1 e2 e3 => expr.If (plug C1 e) e2 e3
+    | If2 e1 C2 e3 => expr.If e1 (plug C2 e) e3
+    | If3 e1 e2 C3 => expr.If e1 e2 (plug C3 e)
+    end.
+End context.
+
+Module context_has_type.
+  Inductive t : list type.t -> context.t -> list type.t -> type.t -> type.t -> Prop :=
+  | hole : forall G ty, t G context.hole G ty ty
+  | abs : forall G' C G ty ty1' ty2',
+      t (ty1' :: G') C (ty1' :: G) ty ty2' ->
+      t G' (context.abs C) (ty1' :: G) ty (type.arrow ty1' ty2')
+  | app1 : forall G' C G ty ty1' ty2' e,
+      t G' C G ty (type.arrow ty1' ty2') ->
+      has_type.t G' e ty1' ->
+      t G' (context.app1 C e) G ty ty2'
+  | app2 : forall G' C G ty ty1' ty2' e,
+      has_type.t G' e (type.arrow ty1' ty2') ->
+      t G' C G ty ty1' ->
+      t G' (context.app2 e C) G ty ty2'
+  | If1 : forall G' C1 G ty ty' e2 e3,
+      t G' C1 G ty type.bool ->
+      has_type.t G' e2 ty' ->
+      has_type.t G' e3 ty' ->
+      t G' (context.If1 C1 e2 e3) G ty ty'
+  | If2 : forall G' C2 G ty ty' e1 e3,
+      has_type.t G' e1 type.bool ->
+      t G' C2 G ty ty' ->
+      has_type.t G' e3 ty' ->
+      t G' (context.If2 e1 C2 e3) G ty ty'
+  | If3 : forall G' C3 G ty ty' e1 e2,
+      has_type.t G' e1 type.bool ->
+      has_type.t G' e2 ty' ->
+      t G' C3 G ty ty' ->
+      t G' (context.If3 e1 e2 C3) G ty ty'
+  .
+
+  Theorem plug :
+    forall G' C G ty ty',
+      t G' C G ty ty' ->
+      forall e,
+        has_type.t G e ty ->
+        has_type.t G' (context.plug C e) ty'.
+  Proof.
+    induction 1; intros e0 HT0; cbn [context.plug]; try assumption;
+      apply IHt in HT0; econstructor; eauto.
+  Qed.
+End context_has_type.
+
+Module context_equiv.
+  Definition t G e1 e2 ty : Prop :=
+    forall C v1 v2,
+      context_has_type.t [] C G ty type.bool ->
+      step.star (context.plug C e1) v1 ->
+      value.t v1 ->
+      step.star (context.plug C e2) v2 ->
+      value.t v2 ->
+      v1 = v2.
+End context_equiv.
+
+End add_valuet_app2.
+
+(*
+ * Effectively, we can think of the addition to the theorem
+ * star_app2 as defining the patch for that case.
+ *)
+
+(*
+ * The commented out terms below are reduced to the same namespace,
+ * and equivalent modules (expr_ast.t and expr.t) are rewritten as the same type
+ * for clarity of differencing.
+ *)
+
+(*
+old.step.star_app2 = 
+  fun (e1 e2 e2' : expr.t) (Star : step.star e2 e2') =>
+    clos_refl_trans_n1_ind
+      expr.t
+      step.t
+      e2
+      (fun (e2'0 : expr.t) =>
+        forall (e3 : expr.t),
+          step.star (expr_ast.app e3 e2) (expr_ast.app e3 e2'0))
+      (fun (e3 : expr.t) =>
+        rtn1_refl expr.t step.t (expr_ast.app e3 e2))
+      (fun (y z : expr.t) (H : step.t y z) (_ : clos_refl_trans_n1 expr.t step.t e2 y)
+           (IHStar : forall (e3 : expr.t), step.star (expr_ast.app e3 e2) (expr_ast.app e3 y)) 
+           (e3 : expr.t) =>
+         Relation_Operators.rtn1_trans
+           expr.t
+           step.t
+           (expr_ast.app e3 e2)
+           (expr_ast.app e3 y)
+           (expr_ast.app e3 z)
+           (step.app2 e3 y z H) 
+           (IHStar e3))
+      e2'
+      Star
+      e1
+: forall (e1 e2 e2' : expr.t),
+    step.star e2 e2' -> step.star (expr_ast.app e1 e2) (expr_ast.app e1 e2')
+ *)
+
+Print add_valuet_beta.step.star_app2.
+
+(*
+add_valuet_beta.step.star_app2 = 
+  fun (e1 e2 e2' : expr.t) (Star : step.star e2 e2') =>
+    clos_refl_trans_n1_ind
+      expr.t
+      step.t
+      e2
+      (fun (e2'0 : expr.t) =>
+        forall (e3 : expr.t),
+        step.star (expr_ast.app e3 e2) (expr_ast.app e3 e2'0))
+      (fun (e3 : expr.t) =>
+        rtn1_refl expr.t step.t (expr_ast.app e3 e2))
+      (fun (y z : expr.t) (H : step.t y z) (_ : clos_refl_trans_n1 expr.t step.t e2 y)
+           (IHStar : forall (e3 : expr.t), step.star (expr_ast.app e3 e2) (expr_ast.app e3 y))
+           (e3 : expr.t) =>
+        Relation_Operators.rtn1_trans
+          expr.t
+          step.t
+          (expr_ast.app e3 e2)
+          (expr_ast.app e3 y)
+          (expr_ast.app e3 z)
+          (step.app2 e3 y z H)
+          (IHStar e3))
+      e2' 
+      Star
+      e1
+: forall (e1 e2 e2' : expr.t),
+    step.star e2 e2' -> step.star (expr_ast.app e1 e2) (expr_ast.app e1 e2')
+*)
+
+Print add_valuet_app2.step.star_app2.
+
+(*
+add_valuet_app2.step.star_app2 =
+  fun (e1 e2 e2' : expr.t) (Val1 : value.t e1) (Star : step.star e2 e2') =>
+    clos_refl_trans_n1_ind
+      expr.t
+      step.t
+      e2
+      (fun (e2'0 : expr.t) =>
+        forall (e3 : expr.t),
+          value.t e3 ->
+          step.star (expr_ast.app e3 e2) (expr_ast.app e3 e2'0))
+      (fun (e3 : expr.t) (_ : value.t e3) =>
+        rtn1_refl expr.t step.t (expr_ast.app e3 e2))
+      (fun (y z : expr.t) (H : step.t y z) (_ : clos_refl_trans_n1 expr.t step.t e2 y)
+           (IHStar : forall (e3 : expr.t), value.t e3 -> step.star (expr_ast.app e3 e2) (expr_ast.app e3 y))
+           (e3 : expr.t)
+           (Val2 : value.t e3) =>
+        Relation_Operators.rtn1_trans
+          expr.t
+          step.t
+          (expr_ast.app e3 e2)
+          (expr_ast.app e3 y)
+          (expr_ast.app e3 z)
+          (step.app2 e3 y z Val2 H) 
+          (IHStar e3 Val2))
+      e2'
+      Star
+      e1
+      Val1
+: forall (e1 e2 e2' : expr.t),
+    value.t e1 ->
+    step.star e2 e2' -> step.star (expr_ast.app e1 e2) (expr_ast.app e1 e2')
+*)
+
+(*
+ * Changes to star_app2:
+ *
+ * 1. New hypothesis Val1 : value.t e1
+ * 2. In definition of P passed to induction principle clos_refl_trans_n1_ind,
+ *    a new hypothesis of type value.t e3, but an otherwise identical case
+ * 3. In base case, a new hypothesis of type value.t e3, but an otherwise identical case
+ * 4. A new hypothesis of type value.t e3 in the induction hypothesis IHStar
+ * 5. A new hypothesis Val2 : value.t e3 in the inductive case
+ * 6. In the body of the inductive case, sticking Val2 into the application of step.app2
+ * 7. Applying the new hypothesis Val1 at the very end
+ * 8. A new hypothesis in of type value.t e1 in the type itself
+ *)
+
+(*
+ * In other words, to construct a new (app2 e3) from an old (app2 e3),
+ * the ornament needs to take in an element of type (value.t e3).
+ * The patch for the ornament constructs a value.t e3 from the context.
+ *
+ * So this isn't quite as interesting as the list case, but what happens here is that
+ * we construct value.t e3 by extending the context. We extend the context
+ * of the property itself to get there, so this change happens universally.
+ * This is a kind of change we can always make when we extend an inductive type in this way,
+ * though it won't always give us an interesting new theorem. It's kind of analogous to this:
+ *)
+
+Definition extend_nat (T : Type) (n : nat) : Type :=
+  nat_rect
+    (fun (_ : nat) => Type)
+    unit
+    (fun (_ : nat) (IH : Type) =>
+      T)
+    n.
+
+Definition extend_nat_next (T : Type) : Type :=
+  forall (n : nat),
+    extend_nat T n ->
+    T ->
+    extend_nat T (S n).
+
+Theorem extend_nat_next_impl :
+  forall (T : Type) (n : nat),
+    extend_nat T n ->
+    T ->
+    extend_nat T (S n).
+Proof.
+  intros T n ext t. apply t.
+Defined.
+
+Theorem extend_nat_impl:
+  forall (T : Type) (n : nat),
+    extend_nat_next T ->
+    T ->
+    extend_nat T n.
+Proof.
+  intros T n next t. induction n.
+  - apply tt.
+  - apply next.
+    + apply IHn.
+    + apply t.
+Defined.
+
+Theorem patch_S (T : Type) :
+  forall (n : nat),
+    extend_nat T (S n) ->
+    extend_nat T n ->
+    (extend_nat T n -> list T) ->
+    list T.
+Proof.
+  intros n ext_S ext IH. apply cons.
+  - apply ext_S.
+  - apply IH. apply ext.
+Defined.
+
+Theorem patch_O (T : Type) :
+  extend_nat T O ->
+  list T.
+Proof.
+  intros ext. apply nil. 
+Defined.
+
+Eval compute in (fun (T : Type) => patch_O T tt).
+
+Eval compute in
+  (fun (T : Type) (t1 : T) =>
+    patch_S T O t1 tt (patch_O T)). 
+
+Theorem foo:
+  forall (T : Type) (t1 t2 : T),
+    list T.
+Proof.
+  intros. apply (patch_S T 1).
+  - apply t1.
+  - apply t2.
+  - intros ext. apply (patch_S T O).
+    + apply ext.
+    + apply tt.
+    + intros ext2. apply patch_O. apply ext2.
+Defined.
+
+Print foo.
+
+Eval compute in
+  (fun (T : Type) (t2 t1 : T) =>
+    patch_S T 1 t2 t1
+      (fun (ext : extend_nat T 1) =>
+         patch_S T 0 ext tt
+           (fun (ext2 : extend_nat T 0) => patch_O T ext2))).
+
+Theorem foo'_inv:
+  forall (T : Type) (l : list T),
+    nat.
+Proof.
+  intros T l. induction l.
+  - apply O.
+  - apply (S IHl).
+Defined.
+
+(*
+ * I got really sidetracked, go figure.
+ * Ignore all of this for now.
+ *)
+
+(*
+ * As a proof this works, but computationally this sucks because it adds the same
+ * t to each inductive case.
+ *
+ * However, if we're proving something about properties, this might
+ * actually make sense. Let's pick some property that lists preserve about nats.
+ *)
+
+Definition P (n : nat) :=
+  0 <= n.
+
+Inductive le_list (T : Type) (l : list T) : list T -> Prop :=
+| le_l : le_list T l l
+| le_cons : forall (l' : list T) (t : T),
+           le_list T l l' ->
+           le_list T l (cons t l').
+
+Definition Q (T : Type) (t : T) (l : list T) :=
+  le_list T nil l.
+
+Theorem bar:
+  forall (n : nat),
+    P n.
+Proof.
+  intros. induction n; unfold P. 
+  - apply le_n. 
+  - apply le_S. apply IHn.
+Defined.
+
+Theorem baz:
+  forall (T : Type) (t : T) (l : list T),
+    Q T t l.
+Proof.
+  intros. induction l; unfold Q.
+  - apply le_l.
+  - apply le_cons. apply IHl.  
+Defined.
+
+Print bar.
+
+(*
+bar = 
+fun n : nat =>
+nat_ind (fun n0 : nat => P n0) (le_n 0)
+  (fun (n0 : nat) (IHn : P n0) => le_S 0 n0 IHn) n
+     : forall n : nat, P n
+ *)
+
+Print baz. 
+
+(*
+ baz = 
+fun (T : Type) (t : T) (l : list T) =>
+list_ind (fun l0 : list T => Q T t l0) (le_l T [])
+  (fun (a : T) (l0 : list T) (IHl : Q T t l0) =>
+   le_cons T [] l0 a IHl) l
+     : forall (T : Type) (t : T) (l : list T), Q T t l
+*)
+
+(*
+ * We don't need a patch at the tactic level for this one because
+ * it's obvious, but probably would if it showed up as a later premise,
+ * which is what happens for James' proof.
+ *)
+
+(*
+ * This just means that expressing the computational patch for lists to nats
+ * that actually takes a different t for each case is harder than this problem.
+ * But for now, maybe we can just solve this problem.
+ *)
+
+(*
+ * OK, but given that people are working at the tactic level, now
+ * what?
+ *
+ * We could define this entire new function for them, but that's lame.
+ *
+ * Probably, honestly, an ad-hoc approach is the best for this.
+ * In other words, use ornaments to search, but don't actually
+ * define them in Coq, or ever. Ornaments just tell us
+ * how to search and apply?
+ *
+ * That is, here, we can tell from the difference in types
+ * that we are looking for an ornament that extends that case.
+ *
+ * So, TODO next time:
+ * 1. Define a patch term that gets you through with the same proof that you can apply in the case.
+ * 2. After, determine how to reconcile that with the theory of ornaments.
+ *)
+
