stlc_unary.v
@@ -1,5 +1,13 @@
 From mm Require Import util stlc.
 
+Module old.
+
+Module expr := stlc.old.expr.
+Module step := stlc.old.step.
+Module value := stlc.old.value.
+Module type := stlc.old.type.
+Module has_type := stlc.old.has_type.
+
 Module terminating.
   Definition t (P : expr.t -> Prop) (e : expr.t) :=
     exists v,
@@ -238,3 +246,503 @@ Proof.
   specialize (SHT [] ltac:(constructor)).
   now rewrite expr.subst_identity with (n := 0) in SHT.
 Qed.
+
+End old.
+
+Module add_valuet_beta.
+
+Module expr := stlc.add_valuet_beta.expr.
+Module step := stlc.add_valuet_beta.step.
+Module value := stlc.add_valuet_beta.value.
+Module type := stlc.add_valuet_beta.type.
+Module has_type := stlc.add_valuet_beta.has_type.
+
+Module terminating.
+  Definition t (P : expr.t -> Prop) (e : expr.t) :=
+    exists v,
+      step.star e v /\
+      value.t v /\
+      P v
+  .
+End terminating.
+
+Fixpoint V ty e :=
+  match ty with
+    | type.bool => e = expr.tt \/ e = expr.ff
+    | type.arrow ty1 ty2 =>
+      expr.wf 0 e /\
+      exists body,
+          e = expr.abs body /\
+          forall e2,
+            V ty1 e2 ->
+            terminating.t (V ty2) (expr.subst [e2] body)
+  end.
+Notation E ty :=
+  (terminating.t (V ty)).
+
+Lemma V_value :
+  forall ty v,
+    V ty v ->
+    value.t v.
+Proof.
+  intros ty v HV.
+  destruct ty; cbn [V] in HV.
+  - intuition; subst; constructor.
+  - destruct HV as [WF [body [E H]]].
+    subst. constructor.
+Qed.
+
+Lemma V_E :
+  forall ty v,
+    V ty v ->
+    E ty v.
+Proof.
+  intros.
+  exists v.
+  intuition.
+  eauto using V_value.
+Qed.
+
+Lemma V_closed :
+  forall ty e,
+    V ty e ->
+    expr.wf 0 e.
+Proof.
+  induction ty; simpl; intuition; subst; simpl; auto.
+Qed.
+
+Lemma V_list_closed :
+  forall G vs,
+    Forall2 V G vs ->
+    Forall (expr.wf 0) vs.
+Proof.
+  intros G vs F.
+  apply Forall_from_nth.
+  intros n e NEe.
+  destruct (Forall2_nth_error2 F NEe) as [ty [NEty Ve]].
+  eauto using V_closed.
+Qed.
+
+Lemma E_step :
+  forall ty e e',
+    step.t e e' ->
+    E ty e' ->
+    E ty e.
+Proof.
+  intros ty e e' S HE.
+  revert ty HE.
+  induction S; intros ty0 [v [Star [Val HV]]]; exists v; intuition.
+  all: eapply step.step_l; eauto.
+Qed.
+
+Lemma E_star :
+  forall ty e e',
+    step.star e e' ->
+    E ty e' ->
+    E ty e.
+Proof.
+  intros ty e e' Star HE.
+  revert ty HE.
+  now induction Star; eauto using E_step.
+Qed.
+
+Module has_sem_type.
+  Definition t G e ty :=
+    expr.wf (length G) e /\
+    forall vs,
+      Forall2 V G vs ->
+      E ty (expr.subst vs e).
+
+  Lemma var :
+    forall G x ty,
+      nth_error G x = Some ty ->
+      t G (expr.var x) ty.
+  Proof.
+    unfold t.
+    intros G x ty NE.
+    do_nth_error_Some.
+    split; [apply H; congruence|].
+    intros vs F.
+    apply V_E.
+    destruct (Forall2_nth_error1 F NE) as [v [NEv Vv]].
+    cbn.
+    now rewrite NEv.
+  Qed.
+
+  Lemma tt :
+    forall G,
+      t G expr.tt type.bool.
+  Proof.
+    unfold t.
+    intros G.
+    split; [exact I|].
+    intros vs F.
+    apply V_E.
+    cbn.
+    intuition.
+  Qed.
+
+  Lemma ff :
+    forall G,
+      t G expr.ff type.bool.
+  Proof.
+    unfold t.
+    intros G.
+    split; [exact I|].
+    intros vs F.
+    apply V_E.
+    cbn.
+    intuition.
+  Qed.
+
+  Lemma abs :
+    forall G e ty1 ty2,
+      t (ty1 :: G) e ty2 ->
+      t G (expr.abs e) (type.arrow ty1 ty2).
+  Proof.
+    unfold t.
+    intros G e ty1 ty2 [WF HT].
+    split; [now auto|].
+    intros vs F.
+    apply V_E.
+    cbn [V].
+    pose proof (Forall2_length F) as EG.
+    cbn [length] in *.
+    split; [apply expr.wf_subst;
+            [now rewrite EG in WF| now firstorder using V_list_closed]|].
+    exists (expr.subst (expr.descend 1 vs) e).
+    split; [now rewrite expr.descend_1|].
+    intros v Vv.
+    rewrite !expr.subst_cons;
+      firstorder using V_list_closed.
+    now rewrite EG in *.
+  Qed.
+
+  Lemma app :
+    forall G e1 e2 ty1 ty2,
+      t G e1 (type.arrow ty1 ty2) ->
+      t G e2 ty1 ->
+      t G (expr.app e1 e2) ty2.
+  Proof.
+    intros G e1 e2 ty1 ty2.
+    intros [WF1 HT1].
+    intros [WF2 HT2].
+    split; [now cbn; auto|].
+    intros vs F.
+
+    cbn [expr.subst].
+    specialize (HT1 vs F).
+    specialize (HT2 vs F).
+    destruct HT1 as [v1 [Star1 [Val1 V1]]].
+    destruct HT2 as [v2 [Star2 [Val2 V2]]].
+    destruct V1 as [WFv1 [body1 [? H1]]].
+    subst v1.
+    eapply E_star; [|now eauto].
+
+    eapply step.star_trans.
+    eapply step.star_app1. now eauto.
+    eapply step.star_trans.
+    eapply step.star_app2. now eauto.
+    eauto using step.step_l, step.beta.
+  Qed.
+
+  Lemma If :
+    forall G e1 e2 e3 ty,
+      t G e1 type.bool ->
+      t G e2 ty ->
+      t G e3 ty ->
+      t G (expr.If e1 e2 e3) ty.
+  Proof.
+    intros G e1 e2 e3 ty.
+    intros [WF1 HT1].
+    intros [WF2 HT2].
+    intros [WF3 HT3].
+    split; [now cbn; auto|].
+    intros vs F.
+
+    cbn [expr.subst].
+    specialize (HT1 vs F).
+    destruct HT1 as [v1 [Star1 [Val1 V1]]].
+    eapply E_star; [apply step.star_If|]; eauto.
+    destruct V1 as [?|?]; subst;
+      (eapply E_step; [constructor|]); auto.
+  Qed.
+End has_sem_type.
+
+Theorem fundamental :
+  forall G e ty,
+    has_type.t G e ty ->
+    has_sem_type.t G e ty.
+Proof.
+  induction 1.
+  - now apply has_sem_type.var.
+  - apply has_sem_type.tt.
+  - apply has_sem_type.ff.
+  - apply has_type.wf in H.
+    apply has_sem_type.abs; auto.
+  - eapply has_sem_type.app; eauto.
+  - apply has_sem_type.If; auto.
+Qed.
+Print Assumptions fundamental.
+
+Theorem fundamental_closed :
+  forall e ty,
+    has_type.t [] e ty ->
+    E ty e.
+Proof.
+  intros e ty HT.
+  destruct (fundamental _ _ _ HT) as [WF SHT].
+  specialize (SHT [] ltac:(constructor)).
+  now rewrite expr.subst_identity with (n := 0) in SHT.
+Qed.
+
+End add_valuet_beta.
+
+Module add_valuet_app2.
+
+Module expr := stlc.add_valuet_app2.expr.
+Module step := stlc.add_valuet_app2.step.
+Module value := stlc.add_valuet_app2.value.
+Module type := stlc.add_valuet_app2.type.
+Module has_type := stlc.add_valuet_app2.has_type.
+
+Module terminating.
+  Definition t (P : expr.t -> Prop) (e : expr.t) :=
+    exists v,
+      step.star e v /\
+      value.t v /\
+      P v
+  .
+End terminating.
+
+Fixpoint V ty e :=
+  match ty with
+    | type.bool => e = expr.tt \/ e = expr.ff
+    | type.arrow ty1 ty2 =>
+      expr.wf 0 e /\
+      exists body,
+          e = expr.abs body /\
+          forall e2,
+            V ty1 e2 ->
+            terminating.t (V ty2) (expr.subst [e2] body)
+  end.
+Notation E ty :=
+  (terminating.t (V ty)).
+
+Lemma V_value :
+  forall ty v,
+    V ty v ->
+    value.t v.
+Proof.
+  intros ty v HV.
+  destruct ty; cbn [V] in HV.
+  - intuition; subst; constructor.
+  - destruct HV as [WF [body [E H]]].
+    subst. constructor.
+Qed.
+
+Lemma V_E :
+  forall ty v,
+    V ty v ->
+    E ty v.
+Proof.
+  intros.
+  exists v.
+  intuition.
+  eauto using V_value.
+Qed.
+
+Lemma V_closed :
+  forall ty e,
+    V ty e ->
+    expr.wf 0 e.
+Proof.
+  induction ty; simpl; intuition; subst; simpl; auto.
+Qed.
+
+Lemma V_list_closed :
+  forall G vs,
+    Forall2 V G vs ->
+    Forall (expr.wf 0) vs.
+Proof.
+  intros G vs F.
+  apply Forall_from_nth.
+  intros n e NEe.
+  destruct (Forall2_nth_error2 F NEe) as [ty [NEty Ve]].
+  eauto using V_closed.
+Qed.
+
+Lemma E_step :
+  forall ty e e',
+    step.t e e' ->
+    E ty e' ->
+    E ty e.
+Proof.
+  intros ty e e' S HE.
+  revert ty HE.
+  induction S; intros ty0 [v [Star [Val HV]]]; exists v; intuition.
+  all: eapply step.step_l; eauto.
+Qed.
+
+Lemma E_star :
+  forall ty e e',
+    step.star e e' ->
+    E ty e' ->
+    E ty e.
+Proof.
+  intros ty e e' Star HE.
+  revert ty HE.
+  now induction Star; eauto using E_step.
+Qed.
+
+Module has_sem_type.
+  Definition t G e ty :=
+    expr.wf (length G) e /\
+    forall vs,
+      Forall2 V G vs ->
+      E ty (expr.subst vs e).
+
+  Lemma var :
+    forall G x ty,
+      nth_error G x = Some ty ->
+      t G (expr.var x) ty.
+  Proof.
+    unfold t.
+    intros G x ty NE.
+    do_nth_error_Some.
+    split; [apply H; congruence|].
+    intros vs F.
+    apply V_E.
+    destruct (Forall2_nth_error1 F NE) as [v [NEv Vv]].
+    cbn.
+    now rewrite NEv.
+  Qed.
+
+  Lemma tt :
+    forall G,
+      t G expr.tt type.bool.
+  Proof.
+    unfold t.
+    intros G.
+    split; [exact I|].
+    intros vs F.
+    apply V_E.
+    cbn.
+    intuition.
+  Qed.
+
+  Lemma ff :
+    forall G,
+      t G expr.ff type.bool.
+  Proof.
+    unfold t.
+    intros G.
+    split; [exact I|].
+    intros vs F.
+    apply V_E.
+    cbn.
+    intuition.
+  Qed.
+
+  Lemma abs :
+    forall G e ty1 ty2,
+      t (ty1 :: G) e ty2 ->
+      t G (expr.abs e) (type.arrow ty1 ty2).
+  Proof.
+    unfold t.
+    intros G e ty1 ty2 [WF HT].
+    split; [now auto|].
+    intros vs F.
+    apply V_E.
+    cbn [V].
+    pose proof (Forall2_length F) as EG.
+    cbn [length] in *.
+    split; [apply expr.wf_subst;
+            [now rewrite EG in WF| now firstorder using V_list_closed]|].
+    exists (expr.subst (expr.descend 1 vs) e).
+    split; [now rewrite expr.descend_1|].
+    intros v Vv.
+    rewrite !expr.subst_cons;
+      firstorder using V_list_closed.
+    now rewrite EG in *.
+  Qed.
+
+  Lemma app :
+    forall G e1 e2 ty1 ty2,
+      t G e1 (type.arrow ty1 ty2) ->
+      t G e2 ty1 ->
+      t G (expr.app e1 e2) ty2.
+  Proof.
+    intros G e1 e2 ty1 ty2.
+    intros [WF1 HT1].
+    intros [WF2 HT2].
+    split; [now cbn; auto|].
+    intros vs F.
+
+    cbn [expr.subst].
+    specialize (HT1 vs F).
+    specialize (HT2 vs F).
+    destruct HT1 as [v1 [Star1 [Val1 V1]]].
+    destruct HT2 as [v2 [Star2 [Val2 V2]]].
+    destruct V1 as [WFv1 [body1 [? H1]]].
+    subst v1.
+    eapply E_star; [|now eauto].
+
+    eapply step.star_trans.
+    eapply step.star_app1. now eauto.
+    eapply step.star_trans.
+    eapply step.star_app2. now eauto.
+    eauto using step.step_l, step.beta.
+  Qed.
+
+  Lemma If :
+    forall G e1 e2 e3 ty,
+      t G e1 type.bool ->
+      t G e2 ty ->
+      t G e3 ty ->
+      t G (expr.If e1 e2 e3) ty.
+  Proof.
+    intros G e1 e2 e3 ty.
+    intros [WF1 HT1].
+    intros [WF2 HT2].
+    intros [WF3 HT3].
+    split; [now cbn; auto|].
+    intros vs F.
+
+    cbn [expr.subst].
+    specialize (HT1 vs F).
+    destruct HT1 as [v1 [Star1 [Val1 V1]]].
+    eapply E_star; [apply step.star_If|]; eauto.
+    destruct V1 as [?|?]; subst;
+      (eapply E_step; [constructor|]); auto.
+  Qed.
+End has_sem_type.
+
+Theorem fundamental :
+  forall G e ty,
+    has_type.t G e ty ->
+    has_sem_type.t G e ty.
+Proof.
+  induction 1.
+  - now apply has_sem_type.var.
+  - apply has_sem_type.tt.
+  - apply has_sem_type.ff.
+  - apply has_type.wf in H.
+    apply has_sem_type.abs; auto.
+  - eapply has_sem_type.app; eauto.
+  - apply has_sem_type.If; auto.
+Qed.
+Print Assumptions fundamental.
+
+Theorem fundamental_closed :
+  forall e ty,
+    has_type.t [] e ty ->
+    E ty e.
+Proof.
+  intros e ty HT.
+  destruct (fundamental _ _ _ HT) as [WF SHT].
+  specialize (SHT [] ltac:(constructor)).
+  now rewrite expr.subst_identity with (n := 0) in SHT.
+Qed.
+
+End add_valuet_app2.
